src/3d/TypeSizes.fsti
@@ -20,6 +20,8 @@ open FStar.Mul
 module H = Hashtable
 module B = Binding
 
+let alignment = option (x:int{x == 1 \/ x == 2 \/ x == 4 \/ x == 8})
+
 type size =
   | Fixed of int
   | WithVariableSuffix of int
@@ -39,6 +41,9 @@ val size_of_typ (env:env_t) (t:typ)
 
 val value_of_const_expr (env:env_t) (e:expr)
   : ML (option (either bool (integer_type & int)))
+
+val field_size_and_alignment (env:env_t) (enclosing_typ:ident) (field_name:ident)
+  : ML (option (size & alignment))
 
 val field_offsets_of_type (env:env_t) (typ:ident)
 : ML (either (list (ident & int)) string)
